\section{Stability of explicit upwind scheme}
	\begin{equation}
		\label{app:for:explicit}
		u_j^{(n+1)} = u_i^{(n)} - C\Big(u_j^{(n)} - u_{j-1}^{(n)}\Big)
	\end{equation}
	Key to the von Neumann's analysis is assuming that the solution to the difference equation is of the form:
	\begin{equation}
		\label{app:for:vnkey}
		u_j^{(n)} = \sigma^ne^{ikx_j}
	\end{equation}
	
	Recall that $e^{ikx_j} = cos(kx_j) + isin(kx_j)$. Substituting \ref{app:for:vnkey} into \ref{app:for:explicit} results in:
	
	\begin{align}
		\begin{split}
			\sigma ^{n+1}e^{ikx_j} = \sigma^{n}{e^{ikx_j}} - C(\sigma ^{n}e^{ikx_j} - \sigma ^{n}e^{ikx_{j-1}}) \\
		\end{split}
	\end{align}
	
	Noting that
	
	\begin{align}
		\begin{split}
			x_{j+1} &= x_j + \Delta x \\
			x_{j-1} &= x_j - \Delta x
		\end{split}
	\end{align}
	
	and dividing through by $u_j^{(n)} = \sigma^ne^{ikx_j}$ we obtain
	
	\begin{align}
		\begin{split}
			\sigma &= 1 - C\Big(1 - \frac{e^{ikx_{j-1}}}{e^{ikx_j}}\Big) \\
			\sigma &= 1 - C\Big(1 - \frac{e^{ik (x_j - \Delta x)}}{e^{ikx_j}}\Big) \\
			\sigma &= 1 - C\Big(1 - \frac{\frac{e^{ikx_j}}{e^{ik\Delta x}}}{e^{ikx_j}}\Big) \\
			\sigma &= 1 - C\Big(1 - \frac{e^{ikx_j}}{e^{ikx_j}e^{ik\Delta x}}\Big) \\
			\sigma &= 1 - C\Big(1 - e^{-ik\Delta x}\Big) \\
		\end{split}
	\end{align}
	
	The method is stable if the amplification factor is less than 1. The magnitude of the amplification factor is:
	
	\begin{align}
		\begin{split}
			\label{app:for:sigmaExplicit}
			|\sigma|^2 &= \Bigg( 1 - C\Big(1 - e^{-ik\Delta x}\Big)\Bigg)^2 \\
			&= \Bigg( 1 - C\Big(1 -\cos(-k\Delta x) + i\sin(-k\Delta x)\Big)\Bigg)^2 \\
			&= \Bigg(1 - C\Big(1 +\cos(k\Delta x)\Big) - iC\sin(k\Delta x)\Bigg)^2 \\	
			&= 1 - 2C\Big(1 + \cos(k\Delta x)\Big) + C^2\Big(1 +\cos(k\Delta x)\Big)^2 + C^2\sin^2(k\Delta x)
		\end{split}
	\end{align} 
	
	but
	
	\begin{align}
		\begin{split}
			\label{app:for:dependencyExplicit}
			1 - 2C\Big(1 + \cos(k\Delta x)\Big) + &C^2\Big(1 +\cos(k\Delta x)\Big)^2 + C^2\sin^2(k\Delta x) = \\&C^2\Bigg(1 - 2\cos(k\Delta x) + \cos^2(k\Delta x)\Bigg) + C^2\sin^2(k\Delta x) \\
			&= C^2(1-2\cos(k\Delta x)) + C^2 \\
			&= 2C^2(1-\cos(k\Delta x)))
		\end{split}
	\end{align} 
	
	Using dependency \ref{app:for:dependencyExplicit} for \ref{app:for:sigmaExplicit} we obtain:
	
	\begin{align}
		\begin{split}
			|\sigma|^2 &= 1 - 2C\Big(1-\cos(k\Delta x)\Big) + 2C^2\Big(1 - \cos(k\Delta x)\Big) \\
			&= 1-2C\Big(1-\cos(k\Delta x)\Big)(1-C)
		\end{split}
	\end{align} 
	
	The method is table if $|\sigma|^2 < 1$, our equation is presented in a following way:
	
	\begin{align}
		\begin{split}
			1-2C\Big(1-\cos(k\Delta x)\Big)(1-C) &< 1 \\
			-2C\Big(1-\cos(k\Delta x)\Big)(1-C) &< 0 \\
			2C\Big(1-\cos(k\Delta x)\Big)(1-C) &>0 \\
		\end{split}
	\end{align} 
	
	Knowing that $ \forall k,  1 \geq \cos(k\Delta x) \geq -1$, we can obtain final result:
	
	\begin{align}
		\begin{split}
			\begin{cases}
				(1-C) <0 \implies C < 1 \\
				C > 0
			\end{cases}
		\end{split}
	\end{align} 
	
	Summarizing $C \in (0, 1)$.
	
	
	